src/Std/Data/DTreeMap/Raw/Basic.lean
@@ -756,6 +756,14 @@ end Const
 def insertMany {ρ} [ForIn Id ρ ((a : α) × β a)] (t : Raw α β cmp) (l : ρ) : Raw α β cmp :=
   letI : Ord α := ⟨cmp⟩; ⟨t.inner.insertMany! l⟩
 
+/--
+Computes the union of the given tree maps. If a key appears in both maps, the entry contains in the second argument will appear in the result.
+
+This function always merges the smaller map into the larger map.
+-/
+def union (t₁ t₂ : Raw α β cmp) : Raw α β cmp :=
+  letI : Ord α := ⟨cmp⟩; ⟨t₁.inner.union! t₂.inner⟩
+
 @[inline, inherit_doc DTreeMap.eraseMany]
 def eraseMany {ρ} [ForIn Id ρ α] (t : Raw α β cmp) (l : ρ) : Raw α β cmp :=
   letI : Ord α := ⟨cmp⟩; ⟨t.inner.eraseMany! l⟩
@@ -771,7 +779,6 @@ def insertMany {ρ} [ForIn Id ρ (α × β)] (t : Raw α β cmp) (l : ρ) : Raw 
 @[inline, inherit_doc DTreeMap.Const.insertManyIfNewUnit]
 def insertManyIfNewUnit {ρ} [ForIn Id ρ α] (t : Raw α Unit cmp) (l : ρ) : Raw α Unit cmp :=
   letI : Ord α := ⟨cmp⟩; ⟨Impl.Const.insertManyIfNewUnit! t.inner l⟩
-
 end Const
 
 instance [Repr α] [(a : α) → Repr (β a)] : Repr (Raw α β cmp) where
